theories/logrel/adequacy.v
@@ -1,0 +1,52 @@
+From main.prelude Require Import imports labels autosubst.
+(* From main.grad_lang Require Import types. *)
+From main.dyn_lang Require Import definition lemmas labels.
+From main.logrel Require Import definition lib.rfn lib.weakestpre.
+
+From iris.si_logic Require Export bi.
+From iris.proofmode Require Import tactics.
+
+Definition RefineL (L : LabelRel) (e e' : expr) : Prop :=
+  ((∃ v, rtc step e (of_val v)) → (∃ v', rtc step e' (of_val v'))) ∧
+  (∀ ℓ, rtc step e (Error ℓ) → ∃ ℓ', L ℓ ℓ' ∧ rtc step e' (Error ℓ')).
+
+Lemma logrel_adequecy L e e' τ
+  (H : open_exprel_typed [] L e e' τ) :
+    RefineL L e e'.
+Proof.
+  rewrite /open_exprel_typed /exprel_typed /rfn in H.
+  specialize (H L (le_permissive_same L) [] []). asimpl in H.
+  rewrite /val_lift_r /lbl_lift_r in H.
+  assert (H' : ⊢ wp (fun v => ⌜∃ v', rtc step_ne e' (of_val v')⌝)
+                    (fun ℓ => ⌜∃ t' ℓ', rtc step_ne e' t' ∧ faulty t' ℓ' ∧ L ℓ ℓ'⌝) e).
+  { iApply wp_impl. iApply H; auto. auto. iIntros (v) "H".
+    iDestruct "H" as (v') "[%H' _]". eauto. } clear H.
+  assert (H := wp_adequacy _ _ _ H'). clear H'.
+  split.
+  - destruct H as [H _]. intros Hev. destruct Hev as [v Hev].
+    rewrite rtc_step_step_ne_to_val in Hev.
+    destruct (H _ Hev) as [v' G].
+    rewrite -rtc_step_step_ne_to_val in G. eauto.
+  - destruct H as [_ H]. intros ℓ Heℓ.
+    destruct (iffLR (rtc_step_step_ne_to_error _ _) Heℓ) as (t' & Htℓ & et'). clear Heℓ.
+    specialize (H t' ℓ Htℓ et'). destruct H as (t'' & ℓ' & He't'' & Hf & HL).
+    exists ℓ'. split; auto. apply rtc_step_step_ne_to_error. eauto.
+Qed.
+
+Definition comb_trans_lblrel (L L' : LabelRel) : LabelRel :=
+  fun ℓ1 ℓ3 => ∃ ℓ2, L ℓ1 ℓ2 ∧ L' ℓ2 ℓ3.
+
+Notation "L ∘ L'" := (comb_trans_lblrel L L').
+
+Lemma refineL_trans (L L' : LabelRel) e1 e2 e3
+  (H12 : RefineL L e1 e2) (H23 : RefineL L' e2 e3) :
+  RefineL (L ∘ L') e1 e3.
+Proof.
+  split.
+  - destruct H12 as [R12 _]; destruct H23 as [R23 _].
+    intro H1. apply R23. apply R12. apply H1.
+  - destruct H12 as [_ R12]; destruct H23 as [_ R23]. intros ℓ1 H1.
+    destruct (R12 ℓ1 H1) as (ℓ2 & L12 & H2). clear R12.
+    destruct (R23 ℓ2 H2) as (ℓ3 & L23 & H3). clear R23.
+    exists ℓ3. split; auto. exists ℓ2. split; auto.
+Qed.
