theories/maps/linker/definition.v
@@ -1,0 +1,46 @@
+From main.prelude Require Import imports labels.
+From main.grad_lang Require Import definition types typing contexts.
+From main.maps Require Import linker.components.
+
+(* Notation gexpr := grad_lang.definition.expr. *)
+(* Notation dexpr := dyn_lang.definition.expr. *)
+(* Notation gVar := grad_lang.definition.Var. *)
+(* Notation gApp := grad_lang.definition.Var. *)
+
+Section linker.
+
+  Context {ν : label} {Hν : NeverOccurs ν}.
+
+  (* todo; generalize to list of labels? *)
+  Definition linker (ℓ : label) (Γ : list type) (τ : type) : ctx :=
+     AppWithList_ctx (wrap_ctx_vars_ascribe_up ℓ Γ)
+  ++ LamN_ctx (length Γ)
+  ++ [ CTX_Ascribe ℓ Unknown τ ].
+
+  Lemma linker_typed ℓ Γ τ :
+    let n := length Γ in
+    typed_ctx (linker ℓ Γ τ) (replicate n Unknown ++ Γ) Unknown
+                             Γ τ.
+  Proof.
+    apply (typed_ctx_compose _ Γ _ _ _ _ (LamN_type (replicate (length Γ) Unknown) τ)).
+    apply AppWithList_ctx_typed'.
+    { apply Forall2_replicate_l. by rewrite /wrap_ctx_vars_ascribe_up imap_length.
+      apply wrap_ctx_vars_ascribe_up_typed. }
+    apply (typed_ctx_compose _ (replicate (length Γ) Unknown ++ Γ) _ _ _ _ τ).
+    rewrite <- (app_nil_l Γ) at 4.
+    apply typed_ctx_app_r. rewrite <- (replicate_length (length Γ) Unknown) at 1.
+    apply LamN_ctx_typed. repeat econstructor.
+  Qed.
+
+
+End linker.
+
+(* Section dyn_emb. *)
+
+(*   Context {ν : label} {Hν : NeverOccurs ν}. *)
+
+(*   Definition import (ℓ : label) (Γ : list type) (τ : type) (e : dexpr) : gexpr := *)
+(*      Wrap_g (Ascribe ℓ Unknown τ ⌜⌜e⌝⌝) *)
+(*        ((fun τ => Lam (Ascribe ℓ τ Unknown (Var 0))) <$> Γ). *)
+
+(* End dyn_emb. *)
